theories/zoo_kcas/kcas_1__opaque.v
@@ -1,6 +1,0 @@
-From zoo_kcas Require Import
-  kcas_1__code.
-
-#[global] Opaque kcas_1٠make.
-#[global] Opaque kcas_1٠get.
-#[global] Opaque kcas_1٠cas.
