theories/zoo_kcas/kcas_2__opaque.v
@@ -1,6 +1,0 @@
-From zoo_kcas Require Import
-  kcas_2__code.
-
-#[global] Opaque kcas_2٠make.
-#[global] Opaque kcas_2٠get.
-#[global] Opaque kcas_2٠cas.
