theories/zoo_mcas/mcas_1__opaque.v
@@ -1,0 +1,6 @@
+From zoo_mcas Require Import
+  mcas_1__code.
+
+#[global] Opaque mcas_1٠make.
+#[global] Opaque mcas_1٠get.
+#[global] Opaque mcas_1٠cas.
