theories/zoo_mcas/mcas_1__types.v
@@ -11,45 +11,45 @@ From zoo Require Import
   options.
 
 Notation "'casn'" := (
-  in_type "zoo_kcas.kcas_1.state" 0
+  in_type "zoo_mcas.mcas_1.state" 0
 )(in custom zoo_field
 ).
 Notation "'before'" := (
-  in_type "zoo_kcas.kcas_1.state" 1
+  in_type "zoo_mcas.mcas_1.state" 1
 )(in custom zoo_field
 ).
 Notation "'after'" := (
-  in_type "zoo_kcas.kcas_1.state" 2
+  in_type "zoo_mcas.mcas_1.state" 2
 )(in custom zoo_field
 ).
 
 Notation "'loc'" := (
-  in_type "zoo_kcas.kcas_1.cas" 0
+  in_type "zoo_mcas.mcas_1.cas" 0
 )(in custom zoo_proj
 ).
 Notation "'state'" := (
-  in_type "zoo_kcas.kcas_1.cas" 1
+  in_type "zoo_mcas.mcas_1.cas" 1
 )(in custom zoo_proj
 ).
 
 Notation "'status'" := (
-  in_type "zoo_kcas.kcas_1.casn" 0
+  in_type "zoo_mcas.mcas_1.casn" 0
 )(in custom zoo_field
 ).
 Notation "'proph'" := (
-  in_type "zoo_kcas.kcas_1.casn" 1
+  in_type "zoo_mcas.mcas_1.casn" 1
 )(in custom zoo_field
 ).
 
 Notation "'Undetermined'" := (
-  in_type "zoo_kcas.kcas_1.status" 0
+  in_type "zoo_mcas.mcas_1.status" 0
 )(in custom zoo_tag
 ).
 Notation "'Before'" := (
-  in_type "zoo_kcas.kcas_1.status" 1
+  in_type "zoo_mcas.mcas_1.status" 1
 )(in custom zoo_tag
 ).
 Notation "'After'" := (
-  in_type "zoo_kcas.kcas_1.status" 2
+  in_type "zoo_mcas.mcas_1.status" 2
 )(in custom zoo_tag
 ).
