theories/zoo_mcas/mcas_2.v
@@ -1,0 +1,11 @@
+From zoo Require Import
+  prelude.
+From zoo_mcas Require Import
+  mcas_2__types.
+From zoo_mcas Require Export
+  mcas_2__code.
+From zoo Require Import
+  options.
+
+From zoo_mcas Require
+  mcas_2__opaque.
