theories/zoo_mcas/mcas_2__opaque.v
@@ -1,0 +1,6 @@
+From zoo_mcas Require Import
+  mcas_2__code.
+
+#[global] Opaque mcas_2٠make.
+#[global] Opaque mcas_2٠get.
+#[global] Opaque mcas_2٠cas.
